# LV2 Host Info Extension
# PROVISIONAL
# Copyright (C) 2009 David Robillard <d@drobilla.net>
#
# Permission is hereby granted, free of charge, to any person obtaining a
# copy of this software and associated documentation files (the "Software"),
# to deal in the Software without restriction, including without limitation
# the rights to use, copy, modify, merge, publish, distribute, sublicense,
# and/or sell copies of the Software, and to permit persons to whom the
# Software is furnished to do so, subject to the following conditions:
# 
# The above copyright notice and this permission notice shall be included
# in all copies or substantial portions of the Software.
# 
# THE SOFTWARE IS PROVIDED "AS IS", WITHOUT WARRANTY OF ANY KIND, EXPRESS OR
# IMPLIED, INCLUDING BUT NOT LIMITED TO THE WARRANTIES OF MERCHANTABILITY,
# FITNESS FOR A PARTICULAR PURPOSE AND NONINFRINGEMENT. IN NO EVENT SHALL
# THE AUTHORS OR COPYRIGHT HOLDERS BE LIABLE FOR ANY CLAIM, DAMAGES OR
# OTHER LIABILITY, WHETHER IN AN ACTION OF CONTRACT, TORT OR OTHERWISE,
# ARISING FROM, OUT OF OR IN CONNECTION WITH THE SOFTWARE OR THE USE OR
# OTHER DEALINGS IN THE SOFTWARE.

@prefix hi:   <http://lv2plug.in/ns/ext/host-info#> .
@prefix lv2:  <http://lv2plug.in/ns/lv2core#> .
@prefix rdf:  <http://www.w3.org/1999/02/22-rdf-syntax-ns#> .
@prefix rdfs: <http://www.w3.org/2000/01/rdf-schema#> .
@prefix owl:  <http://www.w3.org/2002/07/owl#> .
@prefix xsd:  <http://www.w3.org/2001/XMLSchema#> .
@prefix doap: <http://usefulinc.com/ns/doap#> .
@prefix foaf: <http://xmlns.com/foaf/0.1/> .
@prefix amb:  <http://ambisonics.ch/standards/channels/> .

<http://lv2plug.in/ns/ext/host-info> a lv2:Specification ;
	doap:license <http://usefulinc.com/doap/licenses/mit> ;
	doap:name    "LV2 Host Info" ;
	doap:maintainer [
		a foaf:Person ;
		foaf:name     "David Robillard" ;
		foaf:homepage <http://drobilla.net/> ;
		rdfs:seeAlso  <http://drobilla.net/drobilla.rdf>
	] ;
	lv2:documentation """
<p>This specification defines various properties to represent useful information
about LV2 hosts.  Currently, the primary use of this specification is to describe which
extensions are supported by a given host.</p>

<p>The extensions supported by a host can be described like this:</p>
<pre>
@prefix hi: &lt;http://lv2plug.in/ns/ext/host-info#&gt; .

&lt;http://example.org/some-host&gt; a hi:Host ;
	doap:name "Foo Rack" ;
	hi:supportsExtension [
		hi:extension &lt;http://example.org/some-extension&gt; ;
		hi:sinceVersion "1.2.0"
	] .
</pre>
""" .


## Core Classes / Properties

hi:Host a rdfs:Class ;
	rdfs:label "LV2 Host" ;
	rdfs:subClassOf [ a owl:Restriction ;
		owl:onProperty     doap:name ;
		owl:someValuesFrom xsd:string ;
		owl:minCardinality 1 ;
		rdfs:comment "A hi:Host MUST have at least one string doap:name"
	] ;
	rdfs:comment """
An application that supports loading LV2 plugins, or performs other
LV2 related functionality.
""" .

hi:supportsExtension a rdf:Property ;
	rdfs:domain  hi:Host ;
	rdfs:range   hi:ExtensionSupport ;
	rdfs:label   "supports extension" ;
	rdfs:comment "Relates a Host to its ExtensionSupport" .

hi:ExtensionSupport a rdfs:Class ;
	rdfs:label "Extension Support" ;
	rdfs:subClassOf [ a owl:Restriction ;
		owl:onProperty     hi:sinceVersion ;
		owl:someValuesFrom xsd:string ;
		owl:minCardinality 1 ;
		rdfs:comment """
A hi:ExtensionSupport MUST have at least one string hi:sinceVersion
""" ] ;
	rdfs:comment "A description of the support for an extension by a Host" .

hi:extension a rdf:Property ;
	rdfs:domain  hi:ExtensionSupport ;
	rdfs:range   lv2:Specification ;
	rdfs:label   "extension" ;
	rdfs:comment "Indicates the extension supported by a host." .

hi:sinceVersion a rdf:Property ;
	rdfs:domain  hi:ExtensionSupport ;
	rdfs:range   xsd:string ;
	rdfs:label   "since version" ;
	rdfs:comment """
The initial version of a host which supported an extension.
This property MUST always be given
""" .

hi:untilVersion a rdf:Property ;
	rdfs:domain  hi:ExtensionSupport ;
	rdfs:range   xsd:string ;
	rdfs:label   "until version" ;
	rdfs:comment """
The final version of a host which supported an extension.  This property can
be used if support for an extension was discontinued in a host for some reason.
""" .

