# RDF Schema for LV2 plugins
# PROVISIONAL Revision 4
#
# This document describes the classes and properties that are defined by the
# core LV2 specification.  See <http://lv2plug.in> for more information.
# 
# Copyright (C) 2006-2009 Steve Harris, David Robillard
# 
# Permission is hereby granted, free of charge, to any person obtaining a
# copy of this software and associated documentation files (the "Software"),
# to deal in the Software without restriction, including without limitation
# the rights to use, copy, modify, merge, publish, distribute, sublicense,
# and/or sell copies of the Software, and to permit persons to whom the
# Software is furnished to do so, subject to the following conditions:
# 
# The above copyright notice and this permission notice shall be included
# in all copies or substantial portions of the Software.
# 
# THE SOFTWARE IS PROVIDED "AS IS", WITHOUT WARRANTY OF ANY KIND, EXPRESS OR
# IMPLIED, INCLUDING BUT NOT LIMITED TO THE WARRANTIES OF MERCHANTABILITY,
# FITNESS FOR A PARTICULAR PURPOSE AND NONINFRINGEMENT. IN NO EVENT SHALL
# THE AUTHORS OR COPYRIGHT HOLDERS BE LIABLE FOR ANY CLAIM, DAMAGES OR
# OTHER LIABILITY, WHETHER IN AN ACTION OF CONTRACT, TORT OR OTHERWISE,
# ARISING FROM, OUT OF OR IN CONNECTION WITH THE SOFTWARE OR THE USE OR
# OTHER DEALINGS IN THE SOFTWARE.

@prefix lv2:  <http://lv2plug.in/ns/lv2core#> .
@prefix rdf:  <http://www.w3.org/1999/02/22-rdf-syntax-ns#> .
@prefix rdfs: <http://www.w3.org/2000/01/rdf-schema#> .
@prefix owl:  <http://www.w3.org/2002/07/owl#> .
@prefix xsd:  <http://www.w3.org/2001/XMLSchema#> .
@prefix doap: <http://usefulinc.com/ns/doap#> .
@prefix foaf: <http://xmlns.com/foaf/0.1/> .

####################
## Resource Class ##
####################

lv2:Resource a rdfs:Class ;
    rdfs:comment """
An LV2 Resource (e.g. plugin, specification, or any other LV2 related thing)
""" .


#########################
## Specification Class ##
#########################

lv2:Specification a rdfs:Class ;
    rdfs:subClassOf lv2:Resource ;
    rdfs:comment """
An LV2 specification (i.e. this specification, or an LV2 "extension").

Specification data, like plugin data, is distributed in standardized bundles
so hosts may discover all present LV2 data.  See http://lv2plug.in/docs for
more details.
""" .


#######################
## LV2 Specification ##
#######################

<http://lv2plug.in/ns/lv2core>
    a doap:Project , lv2:Specification ;
    doap:license <http://usefulinc.com/doap/licenses/mit> ;
    doap:name "LV2" ;
    doap:homepage <http://lv2plug.in> ;
    doap:created "2004-04-21" ;
    doap:shortdesc "An audio processing plugin specification" ;
    doap:programming-language "C" ;
    doap:release [
        doap:revision "4" ;
        doap:created "2009-08-16"
    ] ;
    doap:maintainer [
        a foaf:Person ;
        foaf:name "Steve Harris" ;
        foaf:homepage <http://plugin.org.uk/> ;
        rdfs:seeAlso <http://plugin.org.uk/swh.xrdf>
    ] , [
        a foaf:Person ;
        foaf:name "David Robillard" ;
        foaf:homepage <http://drobilla.net/> ;
        rdfs:seeAlso <http://drobilla.net/drobilla.rdf>
    ] .



#############################
## Template/Plugin Classes ##
#############################

lv2:Template a rdfs:Class ;
    rdfs:subClassOf lv2:Resource ;
    rdfs:comment """
An abstract plugin-like resource that may not actually be an LV2 plugin
(e.g. may not actually have a plugin binary).  A Template is a Resource
that may have ports, and otherwise mimic the structure of a plugin.
This should be subclassed by extensions that define such things.
""" .
    
lv2:Plugin a rdfs:Class ;
    rdfs:subClassOf lv2:Template ;
    rdfs:label "Plugin" ;
    rdfs:subClassOf [
        a                  owl:Restriction ;
        owl:onProperty     rdf:type ;
        owl:hasValue       lv2:Plugin ;
        rdfs:comment """
A Plugin MUST have at least one rdf:type that is lv2:Plugin.
""" ] , [
        a                  owl:Restriction ;
        owl:onProperty     doap:name ;
        owl:someValuesFrom xsd:string ;
        rdfs:comment """
A Plugin MUST have at least one doap:name that is a string
with no language tag.
""" ] ;
    rdfs:comment """
The class which represents an LV2 plugin.

Plugins SHOULD have a doap:license property whenever possible.
The doap:name property should be at most a few words in length using title
capitalization, e.g. "Tape Delay Unit".  Use doap:shortdesc or
doap:description for more detailed descriptions.
""" .



##################
## Port Classes ##
##################

lv2:Port a rdfs:Class ;
    rdfs:subClassOf lv2:Resource ;
    rdfs:label   "Port" ;
    rdfs:subClassOf [
        a                  owl:Restriction ;
        owl:onProperty     rdf:type ;
        owl:someValuesFrom [
            a         owl:DataRange ;
            owl:oneOf ( lv2:Port lv2:InputPort lv2:OutputPort )
        ] ;
        rdfs:comment """
A Port MUST have at least one rdf:type with object either lv2:Port,
lv2:InputPort, or lv2:OutputPort.
""" ] , [
        a                  owl:Restriction ;
        owl:onProperty     rdf:type ;
        owl:minCardinality 2 ;
        rdfs:comment """
A Port MUST have at least two rdf:type properties with objects that are some
subclass of lv2:Port (one for lv2:Port, lv2:InputPort, or lv2:OutputPort,
and another to describe the specific data type, e.g. lv2:AudioPort).
"""  ] , [
         a                  owl:Restriction ;
         owl:onProperty     lv2:index ;
         owl:someValuesFrom xsd:decimal ;
         owl:cardinality    1 ;
         rdfs:comment """
A port MUST have a single lv2:index which is of type xsd:decimal (e.g. a
literal integer in Turtle).
"""  ] , [
         a                  owl:Restriction ;
         owl:onProperty     lv2:symbol ;
         owl:someValuesFrom xsd:string ;
         rdfs:comment """
A port MUST have a single lv2:symbol which is of type xsd:string with no
language tag.
"""  ] , [
         a                  owl:Restriction ;
         owl:onProperty     lv2:name ;
         owl:someValuesFrom xsd:string ;
         rdfs:comment """
A port MUST have at least one lv2:name which is of type xsd:string.
""" ] ;
    rdfs:comment """
The class which represents an LV2 port.

In order for it to be used by a host it MUST have at least 
the following properties:
    rdf:type (with object one of lv2:Port, lv2:InputPort, lv2:OutputPort)
    rdf:type (more specific port class, see below)
    lv2:index
    lv2:symbol
    lv2:name

All LV2 port descriptions MUST have a property rdf:type where the object is
one of lv2:Port lv2:InputPort or lv2:OutputPort.  Additionally there MUST
be at least one other rdf:type property which more specifically describes
type of the port (e.g. lv2:AudioPort).

Hosts that do not support a specific port class MUST NOT instantiate the
plugin, unless that port has the connectionOptional property set (in which case
the host can simply "connect" that port to NULL).  If a host is interested
in plugins to insert in a certain signal path (e.g. stereo audio), it SHOULD
consider all the classes of a port to determine which ports are most suitable
for connection (e.g. by ignoring ports with additional classes the host does
not recognize).

A port has two identifiers - a (numeric) index, and a (textual) symbol.
The index can be used as an identifier at run-time, but persistent references
to ports (e.g. in a saved preset) MUST use the symbol.  A symbol is guaranteed
to refer to the same port on all plugins with a given URI.  An index does NOT
necessarily refer to the same port on all plugins with a given URI (i.e. the
index for a port may differ between plugin binaries).
""" .

lv2:InputPort a rdfs:Class ;
    rdfs:subClassOf lv2:Port ;
    rdfs:label      "Input port" ;
    rdfs:comment    """
Ports of this type will be connected to a pointer to some value, which will
be read by the plugin during their run method.
""" .

lv2:OutputPort a rdfs:Class ;
    rdfs:subClassOf lv2:Port ;
    rdfs:label      "Output port" ;
    rdfs:comment    """
Ports of this type will be connected to a pointer to some value, which will
be written to by the plugin during their run method.
""" .

lv2:ControlPort a rdfs:Class ;
    rdfs:subClassOf lv2:Port ;
    rdfs:label      "Control port" ;
    rdfs:comment    """
Ports of this type will be connected to a pointer to a single value conforming
to the 32bit IEEE-754 floating point specification.
""" .

lv2:AudioPort a rdfs:Class ;
    rdfs:subClassOf lv2:Port ;
    rdfs:label      "Audio port" ;
    rdfs:comment    """
Ports of this type will be connected to an array of length SampleCount
conforming to the 32bit IEEE-754 floating point specification.
""" .


#####################################
## Mandatory Plugin RDF Properties ##
#####################################

lv2:port a rdf:Property ;
    rdfs:domain  lv2:Template ;
    rdfs:range   lv2:Port ;
    rdfs:label   "port" ;
    rdfs:comment "Relates a Template or Plugin to the Ports it contains" .

lv2:revision a rdf:Property ;
    rdfs:domain lv2:Resource ;
    rdfs:range  xsd:nonNegativeInteger ;
    rdfs:label  "revision" ;
    rdfs:comment """
The revision of an LV2 Resource.  If a plugin's port indices change, the
revision of the plugin MUST be increased.  Note that if port symbols
change or are removed, the plugin URI MUST be changed, the revision acts
as a 'minor version' to distinguish otherwise compatible revisions of
a plugin.  A plugin that has changed indices MUST have a lv2:revision
property, if a plugin has no revision property it is assumed to be 0.

Anything that refers to a specific revision of a plugin (e.g. a serialisation
that depends on specific port indices) MUST refer to the plugin by URI along
with the revision.

This property may be used for other objects, in this case it should be
used in a similar way to represent a 'minor version', and NOT as a major
version to distinguish incompatible objects (use the URI for that).
""" .


####################################
## Optional Plugin RDF Properties ##
####################################

lv2:basicXHTML a rdfs:Class ;
    rdfs:seeAlso <http://www.w3.org/TR/xhtml1/> ;
    rdfs:seeAlso <http://www.w3.org/TR/xhtml-modularization/> ;
    rdfs:comment """
A very basic subset of XHTML for use with lv2:documentation, intended to be
reasonable for hosts to support for styled inline documentation.

A literal with this data type is an XHTML 1.0 fragment containing only
tags from the following XHTML modules: text, hypertext, list, basic tables,
image, presentation.  See the XHTML and XHTML Modularization specifications
for details.  A literal with this data type must be legal to insert as the
body of a &lt;div&gt; tag (free text is allowed).

If only basicXHTML documentation is given but a host has no facilities for
handling tags, simply stripping tags and inserting newlines after appropriate
tags will yield a somewhat readable plain text version of the documentation.
""" .

lv2:documentation a rdf:Property ;
    rdfs:domain  lv2:Resource ;
    rdfs:label   "documentation" ;
    rdfs:comment """
Relates a Plugin to some text/audio/video documentation either online or
included with the plugin package.  The value of this property may be either a
URL, or a literal of any type.  Literal documentation SHOULD be either plain
text, or lv2:basicXHTML.  More advanced documentation should be linked to instead.
""" .



###################################
## Mandatory Port RDF Properties ##
###################################

lv2:index a rdf:Property ;
    rdfs:domain  lv2:Port ;
    rdfs:range   xsd:nonNegativeInteger ;
    rdfs:label   "index" ;
    rdfs:comment """
Specifies the index of the port, passed as an argument to the connect port
function. The index uniqely identifies the port on an instance of the plugin.
""" .

lv2:symbol a rdf:Property ;
    rdfs:domain  lv2:Resource ;
    rdfs:label   "symbol" ;
    rdfs:comment """
A short name used as a machine and human readable identifier.

The first character must be one of _, a-z or A-Z and subsequenct characters can
be from _, a-z, A-Z and 0-9.

A language tag MUST NOT be used on this property.  The symbol uniquely
identifies the port on a plugin with a given URI (i.e. the plugin author MUST
change the plugin URI if a port symbol is changed or removed).
""" .

lv2:name a rdf:Property ;
    rdfs:domain  lv2:Port ;
    rdfs:label   "name" ;
    rdfs:comment """
A display name for labeling the Port in a user interface.

This property is required for Ports, but MUST NOT be used by the host for
port identification. The plugin author may change the values of this
property without changing the Plugin URI.
""" .



##################################
## Optional Port RDF Properties ##
##################################

lv2:Point a rdfs:Class ;
    rdfs:label   "Port value point" ;
    rdfs:comment """
Used to describe interesting values in a Port's range.  To be valid it
requires two properties: rdfs:label and rdf:value.

There are 3 specially defined Points in the LV2 specification (default,
minimum, and maximum), though future extensions may define more.
""" .

lv2:ScalePoint a rdfs:Class ;
    rdfs:subClassOf lv2:Point ;
    rdfs:comment "A single lv2:float Point (for control inputs)" .

lv2:scalePoint a rdf:Property ;
    rdfs:domain  lv2:Port ;
    rdfs:range   lv2:ScalePoint ;
    rdfs:label   "Scale point" ;
    rdfs:comment "Relates a Port to its ScalePoints." .

lv2:default a rdf:Property ;
    rdfs:subPropertyOf lv2:scalePoint ;
    rdfs:label         "Default value" ;
    rdfs:comment """
The default value that the host SHOULD set this port to when there is no
other information available.
""" .

lv2:minimum a rdf:Property ;
    rdfs:subPropertyOf lv2:scalePoint ;
    rdfs:label         "Minimum value" ;
    rdfs:comment """
A hint to the host for the minimum useful value that the port will use.
This is a "soft" limit - the plugin is required to gracefully accept all
values in the range of lv2:float.
""" .

lv2:maximum a rdf:Property ;
    rdfs:subPropertyOf lv2:scalePoint ;
    rdfs:label         "Maximum value" ;
    rdfs:comment """
A hint to the host for the maximum useful value that the port will use.
This is a "soft" limit - the plugin is required to gracefully accept all
values in the range of lv2:float.
""" .



##############
## Features ##
##############

lv2:Feature a rdfs:Class ;
    rdfs:subClassOf lv2:Resource ;
    rdfs:label   "Feature" ;
    rdfs:comment "An additional feature which a plugin may use or require.".

lv2:optionalFeature a rdf:Property ;
    rdfs:domain  lv2:Resource ;
    rdfs:range   lv2:Feature ;
    rdfs:label   "Optional feature" ;
    rdfs:comment """
Signifies that a plugin or other resource supports a certain features.
If the host supports this feature, it MUST pass its URI and any additional
data to the plugin in the instantiate() function. The plugin MUST NOT fail to
instantiate if an optional feature is not supported by the host.
This predicate may be used by extensions for any type of subject.
""" .

lv2:requiredFeature a rdf:Property ;
    rdfs:domain  lv2:Resource ;
    rdfs:range   lv2:Feature ;
    rdfs:label   "Required feature" ;
    rdfs:comment """
Signifies that a plugin or other resource requires a certain feature.
If the host supports this feature, it MUST pass its URI and any additional
data to the plugin in the instantiate() function. The plugin MUST fail to 
instantiate if a required feature is not present; hosts SHOULD always check 
this before attempting to instantiate a plugin (i.e. discovery by attempting 
to instantiate is strongly discouraged).
This predicate may be used by extensions for any type of subject.
""" .


####################
## PortProperties ##
####################

lv2:PortProperty a rdfs:Class ;
    rdfs:label "Port property" ;
    rdfs:comment """
A port property - a useful piece of information that allows a host to make more
sensible decisions (e.g. to provide a better interface).
""" .

lv2:portProperty a rdf:Property ;
    rdfs:domain  lv2:Port ;
    rdfs:range   lv2:PortProperty ;
    rdfs:label   "Port property" ;
    rdfs:comment """
Relates Ports to PortProperties. The PortProperty may be ignored without 
catastrophic effects, though it may be useful e.g. for providing a sensible
interface for the port.
""" .


#######################
## Standard Features ##
#######################

lv2:isLive a lv2:Feature ;
    rdfs:label   "Has a live (realtime) dependency" ;
    rdfs:comment """
Indicates that the plugin has a real-time dependency (e.g. queues data from
a socket) and so its output must not be cached or subject to significant
latency, and calls to the run method should be done in rapid succession.
This property is not related to "hard real-time" execution requirements
(see lv2:hardRTCapable).
""" .

lv2:inPlaceBroken a lv2:Feature ;
    rdfs:label   "in-place broken" ;
    rdfs:comment """
Indicates that the plugin may cease to work correctly if the host elects
to use the same data location for both audio input and audio output.
Plugins that will fail to work correctly if ANY input buffer for a port of
the class lv2:AudioPort is set to the same location as ANY output buffer for
a port of the same class (with connect_port()) MUST require this Feature.
Doing so should be avoided as it makes it impossible for hosts to use the
plugin to process audio "in-place".
""" .

lv2:hardRTCapable a lv2:Feature ;
    rdfs:label   "Hard realtime capable" ;
    rdfs:comment """
Indicates that the plugin is capable of running not only in a conventional host
but also in a "hard real-time" environment. To qualify for this the plugin MUST
satisfy all of the following:

    (1) The plugin must not use malloc(), free() or other heap memory
    management within its Audio class functions. All new memory used in 
    Audio class functions must be managed via the stack. These restrictions 
    only apply to the Audio class functions.

    (2) The plugin will not attempt to make use of any library
    functions in its Audio class functions, with the exceptions of functions 
    in the ANSI standard C and C maths libraries, which the host is expected to
    provide.

    (3) The plugin will not access files, devices, pipes, sockets, IPC
    or any other mechanism that might result in process or thread
    blocking within its Audio class functions.
      
    (4) The plugin will take an amount of time to execute a run() call 
    approximately of form (A+B*SampleCount) where A and B depend on the 
    machine and host in use. This amount of time may not depend on input
    signals or plugin state. The host is left the responsibility to perform 
    timings to estimate upper bounds for A and B. The plugin will also take an
    approximately constant amount of time to execute a connect_port() call.
""" .


#############################
## Standard PortProperties ##
#############################

lv2:connectionOptional a lv2:PortProperty ;
    rdfs:label   "Optionally connected port" ;
    rdfs:comment """
Indicates that this port does not have to be connected to valid data by the
host. If it is to be disconnected then the port MUST set to NULL with a call
to the connectPort method.
""" .

lv2:reportsLatency a lv2:PortProperty ;
    rdfs:label   "Latency reporting port" ;
    rdfs:comment """
Indicates that the port is used to express the processing latency incurred by
the plugin, expressed in samples.  The latency may be affected by the current
sample rate, plugin settings, or other factors, and may be changed by the
plugin at any time.  Where the latency is frequency dependent the plugin may
choose any appropriate value.  If a plugin introduces latency it MUST provide
EXACTLY ONE port with this property set which informs the host of the "correct" 
latency.  In "fuzzy" cases the value output should be the most reasonable based
on user expectation of input/output alignment (eg. musical delay/echo plugins
should not report their delay as latency, as it is an intentional effect).
""" .

lv2:toggled a lv2:PortProperty ;
    rdfs:label   "Toggled" ;
    rdfs:comment """
Indicates that the data item should be considered a Boolean toggle. Data less
than or equal to zero should be considered "off" or "false", and data above
zero should be considered "on" or "true".
""" .

lv2:sampleRate a lv2:PortProperty ;
    rdfs:label   "Sample rate" ;
    rdfs:comment """
Indicates that any bounds specified should be interpreted as multiples of the
sample rate. For instance, a frequency range from 0Hz to the Nyquist frequency
(half the sample rate) could be requested by this property in conjunction with
lv2:minimum 0.0 and lv2:maximum 0.5.
Hosts that support bounds at all MUST support this property.
""" .

lv2:integer a lv2:PortProperty ;
    rdfs:label   "Integer" ;
    rdfs:comment """
Indicates that a port's reasonable values are integers (eg. a user interface
would likely wish to provide a stepped control allowing only integer input).
A plugin MUST operate reasonably even if such a port has a non-integer input.
""" .

lv2:enumeration a lv2:PortProperty ;
    rdfs:label   "Enumeration" ;
    rdfs:comment """
Indicates that a port's only reasonable values are the scale points defined for
that port.  Though a host SHOULD NOT allow a user to set the value of such a 
port to anything other than a scale point.  A plugin MUST operate reasonably
even if such a port has an input that is not a scale point, preferably by
simply choosing the largest enumeration value less than or equal to the
actual input value (i.e. round the input value down).
""" .



####################
## Plugin Classes ##
####################

lv2:GeneratorPlugin a rdfs:Class ;
    rdfs:subClassOf lv2:Plugin ;
    rdfs:label "Generator" ;
    rdfs:comment """
Any plugin that generates sound internally, rather than processing its input.
""" .

lv2:InstrumentPlugin a rdfs:Class ;
    rdfs:subClassOf lv2:GeneratorPlugin ;
    rdfs:label "Instrument" ;
    rdfs:comment """
Any plugin that is intended to be played as a musical instrument.
""" .

lv2:OscillatorPlugin a rdfs:Class ;
    rdfs:subClassOf lv2:GeneratorPlugin ;
    rdfs:label "Oscillator" .

lv2:UtilityPlugin a rdfs:Class ;
    rdfs:subClassOf lv2:Plugin ;
    rdfs:label "Utility" ;
    rdfs:comment """
Includes things like mathematical functions and non-musical delays.
""" .

lv2:ConverterPlugin a rdfs:Class ;
    rdfs:subClassOf lv2:UtilityPlugin ;
    rdfs:label "Converter" ;
    rdfs:comment """
Any plugin that converts some form of input into a different form of output.
""" .

lv2:AnalyserPlugin a rdfs:Class ;
    rdfs:subClassOf lv2:UtilityPlugin ;
    rdfs:label "Analyser" ;
    rdfs:comment """
Any plugin that analyses input to output some useful information.
""" .

lv2:MixerPlugin a rdfs:Class ;
    rdfs:subClassOf lv2:UtilityPlugin ;
    rdfs:label "Mixer" ;
    rdfs:comment """
A plugin which mixes some number of inputs into some number of outputs.
""" .

lv2:SimulatorPlugin a rdfs:Class ;
    rdfs:subClassOf lv2:Plugin ;
    rdfs:label "Simulator" ;
    rdfs:comment """
Plugins that aim to duplicate the effect of some environmental effect or
musical equipment.
""" .

lv2:DelayPlugin a rdfs:Class ;
    rdfs:subClassOf lv2:Plugin ;
    rdfs:label "Delay" ;
    rdfs:comment """
Plugins that intentionally delay their input signal as an effect.
""" .

lv2:ModulatorPlugin a rdfs:Class ;
    rdfs:subClassOf lv2:Plugin ;
    rdfs:label "Modulator" .

lv2:ReverbPlugin a rdfs:Class ;
    rdfs:subClassOf lv2:Plugin ;
    rdfs:subClassOf lv2:SimulatorPlugin ;
    rdfs:subClassOf lv2:DelayPlugin ;
    rdfs:label "Reverb" .

lv2:PhaserPlugin a rdfs:Class ;
    rdfs:subClassOf lv2:ModulatorPlugin ;
    rdfs:label "Phaser" .

lv2:FlangerPlugin a rdfs:Class ;
    rdfs:subClassOf lv2:ModulatorPlugin ;
    rdfs:label "Flanger" .

lv2:ChorusPlugin a rdfs:Class ;
    rdfs:subClassOf lv2:ModulatorPlugin ;
    rdfs:label "Chorus" .

lv2:FilterPlugin a rdfs:Class ;
    rdfs:subClassOf lv2:Plugin ;
    rdfs:label "Filter" .

lv2:LowpassPlugin a rdfs:Class ;
    rdfs:subClassOf lv2:FilterPlugin ;
    rdfs:label "Lowpass" .

lv2:BandpassPlugin a rdfs:Class ;
    rdfs:subClassOf lv2:FilterPlugin ;
    rdfs:label "Bandpass" .

lv2:HighpassPlugin a rdfs:Class ;
    rdfs:subClassOf lv2:FilterPlugin ;
    rdfs:label "Highpass" .

lv2:CombPlugin a rdfs:Class ;
    rdfs:subClassOf lv2:FilterPlugin ;
    rdfs:label "Comb" .

lv2:AllpassPlugin a rdfs:Class ;
    rdfs:subClassOf lv2:FilterPlugin ;
    rdfs:label "Allpass" .

lv2:EQPlugin a rdfs:Class ;
    rdfs:subClassOf lv2:FilterPlugin ;
    rdfs:label "Equaliser" .

lv2:ParaEQPlugin a rdfs:Class ;
    rdfs:subClassOf lv2:EQPlugin ;
    rdfs:label "Parametric" .

lv2:MultiEQPlugin a rdfs:Class ;
    rdfs:subClassOf lv2:EQPlugin ;
    rdfs:label "Multiband" .

lv2:SpectralPlugin a rdfs:Class ;
    rdfs:subClassOf lv2:Plugin ;
    rdfs:label "Spectral Processor" .

lv2:PitchPlugin a rdfs:Class ;
    rdfs:subClassOf lv2:SpectralPlugin ;
    rdfs:label "Pitch Shifter" .

lv2:AmplifierPlugin a rdfs:Class ;
    rdfs:subClassOf lv2:Plugin ;
    rdfs:label "Amplifier" .

lv2:DistortionPlugin a rdfs:Class ;
    rdfs:subClassOf lv2:Plugin ;
    rdfs:label "Distortion" .

lv2:WaveshaperPlugin a rdfs:Class ;
    rdfs:subClassOf lv2:DistortionPlugin ;
    rdfs:label "Waveshaper" .

lv2:DynamicsPlugin a rdfs:Class ;
    rdfs:subClassOf lv2:Plugin ;
    rdfs:label "Dynamics Processor" ;
    rdfs:comment """
Plugins that alter the envelope or dynamic range of the processed audio.
""" .

lv2:CompressorPlugin a rdfs:Class ;
    rdfs:subClassOf lv2:DynamicsPlugin ;
    rdfs:label "Compressor" .

lv2:ExpanderPlugin a rdfs:Class ;
    rdfs:subClassOf lv2:DynamicsPlugin ;
    rdfs:label "Expander" .

lv2:LimiterPlugin a rdfs:Class ;
    rdfs:subClassOf lv2:DynamicsPlugin ;
    rdfs:label "Limiter" .

lv2:GatePlugin a rdfs:Class ;
    rdfs:subClassOf lv2:DynamicsPlugin ;
    rdfs:label "Gate" .
