# LV2 Presets Extension
# PROVISIONAL
# Copyright (C) 2009 David Robillard <d@drobilla.net>
#
# Permission is hereby granted, free of charge, to any person obtaining a
# copy of this software and associated documentation files (the "Software"),
# to deal in the Software without restriction, including without limitation
# the rights to use, copy, modify, merge, publish, distribute, sublicense,
# and/or sell copies of the Software, and to permit persons to whom the
# Software is furnished to do so, subject to the following conditions:
# 
# The above copyright notice and this permission notice shall be included
# in all copies or substantial portions of the Software.
# 
# THE SOFTWARE IS PROVIDED "AS IS", WITHOUT WARRANTY OF ANY KIND, EXPRESS OR
# IMPLIED, INCLUDING BUT NOT LIMITED TO THE WARRANTIES OF MERCHANTABILITY,
# FITNESS FOR A PARTICULAR PURPOSE AND NONINFRINGEMENT. IN NO EVENT SHALL
# THE AUTHORS OR COPYRIGHT HOLDERS BE LIABLE FOR ANY CLAIM, DAMAGES OR
# OTHER LIABILITY, WHETHER IN AN ACTION OF CONTRACT, TORT OR OTHERWISE,
# ARISING FROM, OUT OF OR IN CONNECTION WITH THE SOFTWARE OR THE USE OR
# OTHER DEALINGS IN THE SOFTWARE.

@prefix pset: <http://lv2plug.in/ns/ext/presets#> .
@prefix lv2:  <http://lv2plug.in/ns/lv2core#> .
@prefix rdf:  <http://www.w3.org/1999/02/22-rdf-syntax-ns#> .
@prefix rdfs: <http://www.w3.org/2000/01/rdf-schema#> .
@prefix owl:  <http://www.w3.org/2002/07/owl#> .
@prefix xsd:  <http://www.w3.org/2001/XMLSchema#> .
@prefix doap: <http://usefulinc.com/ns/doap#> .
@prefix foaf: <http://xmlns.com/foaf/0.1/> .

<http://lv2plug.in/ns/ext/presets> a lv2:Specification ;
	doap:license <http://usefulinc.com/doap/licenses/mit> ;
	doap:name    "LV2 Presets" ;
	doap:release [
		doap:revision "2.1pre1" ;
		doap:created "2010-10-29"
	] ;
	doap:maintainer [
		a foaf:Person ;
		foaf:name     "David Robillard" ;
		foaf:homepage <http://drobilla.net/> ;
		rdfs:seeAlso  <http://drobilla.net/drobilla.rdf>
	] ;
	rdfs:comment """
Defines presets (e.g. named sets of control values) for LV2 plugins.
""" .

pset:Preset a rdfs:Class ;
    rdfs:subClassOf lv2:PluginBase ;
	rdfs:label "LV2 Preset" ;
	rdfs:comment """
A Preset for an LV2 Plugin.  A preset can be considered an "overlay" on a
Plugin.  Rather than attempting to define all valid predicates for a Preset
(which is not possible since presets may need to specify values for things
defined in other extensions), the presets extension simply provides this
class which can be augmented with any data in the exact same fashion as the
definition of a Plugin.

A Preset SHOULD have at least one pset:appliesTo property.
Each Port on a Preset MUST have at least a lv2:symbol property and a
pset:value property.
""" .

pset:appliesTo a rdf:Property ;
	rdfs:domain  pset:Preset ;
	rdfs:range   lv2:Plugin ;
	rdfs:label   "Applies to" ;
	rdfs:comment """
Specifies the Plugin(s) a Preset may be applied to.  When a Preset applies
to a Plugin, that Preset SHOULD have ports for every control port on that
plugin, each of which SHOULD have a pset:value property.  If the Preset is
missing ports, or refers to ports which do not exist on the Plugin, then
the host SHOULD apply all the values in the preset that do match the Plugin.

The Preset MAY have any other values that should be applied to the Plugin
in some way.  The host SHOULD simply ignore any values on a Preset it does
not understand.
""" .

pset:value a rdf:Property ;
	rdfs:domain  lv2:Port ;
	rdfs:label   "Has value" ;
	rdfs:comment """
Specifies the value of a Port on some Preset.  This property is used
in a similar way to e.g. lv2:default.
""" .

